PMA QED

code/ecdsap256/dist/Hacl_P256.h
@@ -31,6 +31,7 @@
 
 
 #include "Hacl_Kremlib.h"
+#include "Hacl_Lib.h"
 
 /*
  Input: result: uint8[64], 
@@ -57,6 +58,9 @@ bool Hacl_P256_ecp256dh_i(uint8_t *result, uint8_t *scalar);
 */
 bool Hacl_P256_ecp256dh_r(uint8_t *result, uint8_t *pubKey, uint8_t *scalar);
 
+uint32_t Hacl_P256_getScalar(Lib_Buffer_buftype a, void *scalar, uint32_t i);
+
+void brTu(uint8_t *s, uint8_t *newScalar);
 
 #define __Hacl_P256_H_DEFINED
 #endif
