code/ecdsap256/runme.py
@@ -1,0 +1,98 @@
+import os
+
+def writeResult(s):
+    w = genFileW()
+    f = open("/home/nkulatov/master/hacl-star/code/ecdsap256/dist/log", "a+")
+    toWrite = s + "\n" + w + "\n \n"
+    f.write(toWrite)
+    print(toWrite)
+
+def genFileW():
+    i = printInline()
+    loc = computeLOC()
+    return (i + "Lines of code: \n" + loc)
+
+def computeInline():
+    f = open("/home/nkulatov/master/hacl-star/code/ecdsap256/dist/Hacl_P256.c", "r")
+    ff = f.read()
+    index = 0
+    s = ""
+    while (index != -1):
+        index = ff.find("inline", index + 1)
+        index2 = ff.find("\n", index)
+        s = s + ff[index: index2:] + "\n"
+
+    return s
+
+def printInline():
+    return ("Inlined functions in the code: \n") + computeInline()
+
+def makeInt(output):
+    return [int(s) for s in output.split() if s.isdigit()][0]
+
+def readLastLOC():
+    f = open("/home/nkulatov/master/hacl-star/code/ecdsap256/dist/log", "r")
+    ff = f.read()
+    index = 0
+    index2 = 0
+    index3 = 0
+
+    while (index != -1):
+        index = ff.find("Lines of code:", index + 1)
+        if index != -1:
+         index2 = index
+        index3 = ff.find(" ", index)
+
+    return(makeInt(ff[index2: index3]))
+
+
+def computeLOC():
+    stream = os.popen('wc -l ./dist/Hacl_P256.c')
+    output = stream.read() 
+    locNow = makeInt(output)
+
+    locBefore = readLastLOC()
+
+    try:
+        locDiff = locNow - locBefore
+    except Exception as e:
+        locDiff = 0
+
+    sign = ""
+
+    if locDiff >0:
+        sign = "+"
+    elif locDiff < 0:
+        sign = "-"
+
+
+    return str(makeInt(output)) + "  (" + sign + " " + str(locDiff) + ") "
+
+
+
+def readLast():
+    f = open("/home/nkulatov/master/hacl-star/code/ecdsap256/dist/log", "r")
+    ff = f.read()
+    index = 0
+    index2 = 0
+    index3 = 0
+
+    while (index != -1):
+        index = ff.find("bw   ", index + 1)
+        if index != -1:
+            index2 = index
+            index3 = ff.find("Lines", index)
+
+    print("The previous parameters: \n" + ff[index2: index3])
+
+
+if __name__ == '__main__':
+    stream = os.popen('make dist/test.exe')
+    output = stream.read()
+    stream = os.popen('./dist/test.exe')
+    output = stream.read()
+
+    l = writeResult(output)
+
+    readLast()
+
