code/ecdsap256/Hacl.Impl.P256.MixedPointAdd.fst
@@ -5,100 +5,215 @@ open FStar.HyperStack
 module ST = FStar.HyperStack.ST
 
 open Lib.IntTypes
+open Hacl.Impl.P256.Arithmetics
+
 open Lib.Buffer
 
-open Spec.P256.Definitions
 open Spec.P256.Lemmas
+open Spec.P256.Definitions
+open Hacl.Impl.SolinasReduction
+open Spec.P256.MontgomeryMultiplication
+open Spec.P256.MontgomeryMultiplication.PointAdd
+open Hacl.Impl.P256.LowLevel 
+open Hacl.Impl.P256.LowLevel.PrimeSpecific
+open Hacl.Impl.P256.MontgomeryMultiplication
+open Spec.P256
+open Hacl.Impl.P256.Math 
 
-open FStar.Math
+open FStar.Tactics 
+open FStar.Tactics.Canon
+
 open FStar.Math.Lemmas
+
 open FStar.Mul
 
-open Hacl.Impl.P256.LowLevel
-open Hacl.Impl.P256.PointAdd
-
-open Hacl.Impl.P256.MontgomeryMultiplication
-open Hacl.Impl.P256.LowLevel.PrimeSpecific
-
-open Spec.P256.MontgomeryMultiplication
-
-#set-options "--z3rlimit 100 --fuel 0 --ifuel 0"
-
-(* just changing argument order *)
-inline_for_extraction noextract
-val montgomery_multiplication_buffer: result: felem -> a: felem -> b: felem ->  Stack unit
-  (requires (fun h -> live h a /\  as_nat h a < prime256 /\ live h b /\ live h result /\ as_nat h b < prime256)) 
-  (ensures (fun h0 _ h1 -> 
-    modifies (loc result) h0 h1 /\  
-    as_nat h1 result < prime256 /\
-    as_nat h1 result = (as_nat h0 a * as_nat h0 b * modp_inv2_prime (pow2 256) prime256) % prime256 /\
-    as_nat h1 result = toDomain_ (fromDomain_ (as_nat h0 a) * fromDomain_ (as_nat h0 b) % prime256) /\
-    as_nat h1 result = toDomain_ (fromDomain_ (as_nat h0 a) * fromDomain_ (as_nat h0 b)))
-  )
-
-let montgomery_multiplication_buffer result a b = 
-  Hacl.Impl.P256.MontgomeryMultiplication.montgomery_multiplication_buffer a b result
+friend Hacl.Impl.P256.PointAdd
 
 
-inline_for_extraction noextract
-val p256_add: out: felem -> arg1: felem -> arg2: felem -> Stack unit 
-  (requires (fun h0 ->  
-    live h0 arg1 /\ live h0 arg2 /\ live h0 out /\ 
-    eq_or_disjoint arg1 out /\ eq_or_disjoint arg2 out /\
-    as_nat h0 arg1 < prime256 /\ as_nat h0 arg2 < prime256))
-  (ensures (fun h0 _ h1 -> modifies (loc out) h0 h1 /\ 
-      as_nat h1 out == (as_nat h0 arg1 + as_nat h0 arg2) % prime256 /\
-      as_nat h1 out == toDomain_ ((fromDomain_ (as_nat h0 arg1) + fromDomain_ (as_nat h0 arg2)) % prime256)))
-
-let p256_add result a b = Hacl.Impl.P256.LowLevel.PrimeSpecific.p256_add a b result
-
-
-inline_for_extraction noextract
-val p256_double: out: felem -> arg1: felem -> Stack unit 
-  (requires (fun h0 ->  live h0 arg1 /\ live h0 out /\ eq_or_disjoint arg1 out /\ as_nat h0 arg1 < prime256))
-  (ensures (fun h0 _ h1 -> modifies (loc out) h0 h1 /\ 
-    as_nat h1 out == (2 * as_nat h0 arg1) % prime256 /\ as_nat h1 out < prime256 /\
-    as_nat h1 out == toDomain_ (2 * fromDomain_ (as_nat h0 arg1) % prime256)
-  )
-)
-
-let p256_double result a =  Hacl.Impl.P256.LowLevel.PrimeSpecific.p256_double a result
-
-
-inline_for_extraction noextract
-val p256_sub: out: felem -> arg1: felem -> arg2: felem -> Stack unit 
-  (requires 
-    (fun h0 -> live h0 out /\ live h0 arg1 /\ live h0 arg2 /\ 
-      eq_or_disjoint arg1 out /\ eq_or_disjoint arg2 out /\
-      as_nat h0 arg1 < prime256 /\ as_nat h0 arg2 < prime256))
-    (ensures (fun h0 _ h1 -> modifies (loc out) h0 h1 /\ 
-	as_nat h1 out == (as_nat h0 arg1 - as_nat h0 arg2) % prime256 /\
-	as_nat h1 out == toDomain_ ((fromDomain_ (as_nat h0 arg1) - fromDomain_ (as_nat h0 arg2)) % prime256)
-    )
-)    
-
-let p256_sub result a b = Hacl.Impl.P256.LowLevel.PrimeSpecific.p256_sub a b result
-
-
-
-
-inline_for_extraction
-type pointAffine = lbuffer uint64 (size 8)
+#set-options "--z3rlimit 300 --fuel 0 --ifuel 0"
 
 val pointAffineIsNotZero: p: pointAffine -> Stack uint64
-  (requires fun h -> live h p)
+  (requires fun h -> live h p /\ (
+    let x = as_nat h (gsub p (size 0) (size 4)) in 
+    let y = as_nat h (gsub p (size 4) (size 4)) in 
+    x < prime256 /\ y < prime256))
   (ensures fun h0 r h1 -> modifies0 h0 h1 /\ (
-    let x = gsub p (size 0) (size 4) in 
-    let y = gsub p (size 4) (size 4) in 
-    if as_nat h0 x = 0 || as_nat h0 y = 0 then uint_v r = pow2 64 - 1 else uint_v r == 0))
+    let x = as_nat h0 (gsub p (size 0) (size 4)) in 
+    let y = as_nat h0 (gsub p (size 4) (size 4)) in 
+    if isPointAtInfinityAffine (x, y) then uint_v r = pow2 64 - 1 else uint_v r == 0))
 
 let pointAffineIsNotZero p = 
   let x = sub p (size 0) (size 4) in 
   let y = sub p (size 4) (size 4) in 
   let xZero = isZero_uint64_CT x in 
   let yZero = isZero_uint64_CT y in 
-  logor_lemma xZero yZero;
-  logor xZero yZero
+  logand_lemma xZero yZero;
+  logand xZero yZero
+
+
+val pointJacobianIsNotZero: p: point -> Stack uint64
+  (requires fun h -> True)
+  (ensures fun h0 _ h1 -> True)
+
+
+let pointJacobianIsNotZero p = u64 0
+
+
+inline_for_extraction noextract 
+val move_from_jacobian_coordinates_mixed: u1: felem -> u2: felem -> s1: felem -> s2: felem 
+  ->  p: point -> q: pointAffine -> tempBuffer16: lbuffer uint64 (size 16) -> 
+  Stack unit (requires fun h -> live h u1 /\ live h u2 /\ live h s1 /\ live h s2 /\ live h p /\ live h q /\ live h tempBuffer16 /\
+   LowStar.Monotonic.Buffer.all_disjoint [loc tempBuffer16; loc p; loc q; loc u1; loc u2; loc s1; loc s2] /\
+    as_nat h (gsub p (size 8) (size 4)) < prime /\ 
+    as_nat h (gsub p (size 0) (size 4)) < prime /\ 
+    as_nat h (gsub p (size 4) (size 4)) < prime /\ 
+    as_nat h (gsub q (size 0) (size 4)) < prime /\ 
+    as_nat h (gsub q (size 4) (size 4)) < prime
+    )
+  (ensures fun h0 _ h1 ->  
+    modifies (loc u1 |+| loc u2 |+| loc s1 |+| loc s2 |+| loc tempBuffer16) h0 h1  /\
+    as_nat h1 u1 < prime /\ as_nat h1 u2 < prime /\ as_nat h1 s1 < prime /\ as_nat h1 s2 < prime  /\
+    (
+      let pX, pY, pZ = as_nat h0 (gsub p (size 0) (size 4)), as_nat h0 (gsub p (size 4) (size 4)), as_nat h0 (gsub p (size 8) (size 4)) in 
+      let qX, qY = as_nat h0 (gsub q (size 0) (size 4)), as_nat h0 (gsub q (size 4) (size 4)) in 
+      
+      let pxD, pyD, pzD = fromDomain_ pX, fromDomain_ pY, fromDomain_ pZ in 
+      let qxD, qyD = fromDomain_ qX, fromDomain_ qY in 
+  
+      as_nat h1 u1 == toDomain_ (pxD % prime256) /\
+      as_nat h1 u2 == toDomain_ (pzD * pzD * qxD % prime256) /\ 
+      as_nat h1 s1 == toDomain_ (pyD % prime256) /\
+      as_nat h1 s2 == toDomain_ (pzD * pzD * pzD * qyD % prime256)
+))
+
+
+let move_from_jacobian_coordinates_mixed u1 u2 s1 s2 p q tempBuffer = 
+    let h0 = ST.get() in 
+   let pX = sub p (size 0) (size 4) in 
+   let pY = sub p (size 4) (size 4) in 
+   let pZ = sub p (size 8) (size 4) in 
+
+   let qX = sub q (size 0) (size 4) in 
+   let qY = sub q (size 4) (size 4) in 
+
+   let z1Square = sub tempBuffer (size 4) (size 4) in 
+   let z1Cube = sub tempBuffer (size 12) (size 4) in  
+
+   montgomery_square_buffer pZ z1Square;
+   montgomery_multiplication_buffer z1Square pZ z1Cube;
+
+   copy u1 pX;
+   montgomery_multiplication_buffer z1Square qX u2;
+
+   copy s1 pY;
+   montgomery_multiplication_buffer z1Cube qY s2;
+
+  let h1 = ST.get() in 
+  
+  let pX_, pY_ = as_nat h0 (gsub p (size 0) (size 4)), as_nat h0 (gsub p (size 4) (size 4)) in 
+  
+  lemmaFromDomainToDomain (as_nat h1 u1);
+  lemmaFromDomainToDomain (as_nat h1 s1);
+  inDomain_mod_is_not_mod (1 * 1 * fromDomain_ pX_);  
+  inDomain_mod_is_not_mod (1 * 1 * 1 * fromDomain_ pY_);  
+
+  lemma_mod_mul_distr_l (fromDomain_ (as_nat h0 pZ) * fromDomain_ (as_nat h0 pZ)) (fromDomain_ (as_nat h0 pZ)) prime256;
+  lemma_mod_mul_distr_l (fromDomain_ (as_nat h0 pZ) * fromDomain_ (as_nat h0 pZ)) (fromDomain_ (as_nat h0 qX)) prime256;
+  lemma_mod_mul_distr_l 1 (fromDomain_ (as_nat h0 pY)) prime256;
+  lemma_mod_mul_distr_l (fromDomain_ (as_nat h0 pZ) * fromDomain_ (as_nat h0 pZ) * fromDomain_ (as_nat h0 pZ)) (fromDomain_ (as_nat h0 qY)) prime256
+
+
+
+inline_for_extraction noextract 
+val computeZ3_point_add_mixed: z3: felem -> z1: felem -> h: felem -> 
+  Stack unit (requires fun h0 -> live h0 z3 /\ live h0 z1 /\ live h0 h /\
+  as_nat h0 z1 < prime  /\ as_nat h0 h < prime)
+  (ensures fun h0 _ h1 -> modifies (loc z3) h0 h1 /\ as_nat h1 z3 < prime /\ 
+    (
+      let z1D = fromDomain_ (as_nat h0 z1) in 
+      let hD = fromDomain_ (as_nat h0 h) in 
+      as_nat h1 z3 == toDomain_ (z1D * 1 * hD % prime256)
+    )  
+  )  
+
+let computeZ3_point_add_mixed z3 z1 h = 
+    let h0 = ST.get() in 
+  montgomery_multiplication_buffer z1 h z3;
+    lemma_mod_mul_distr_l (fromDomain_ (as_nat h0 z1) * 1) (fromDomain_ (as_nat h0 h)) prime256
+
+
+inline_for_extraction noextract 
+val point_add_if_second_branch_impl: result: point -> p: point 
+  -> q: pointAffine -> u1: felem -> u2: felem -> s1: felem -> 
+  s2: felem -> r: felem -> h: felem -> uh: felem -> hCube: felem -> tempBuffer28 : lbuffer uint64 (size 28) -> 
+  Stack unit 
+    (requires fun h0 -> live h0 result /\ live h0 p /\ live h0 q /\ live h0 u1 /\ live h0 u2 /\ live h0 s1 /\ live h0 s2 /\ live h0 r /\ live h0 h /\ live h0 uh /\ live h0 hCube /\ live h0 tempBuffer28 /\
+    
+    as_nat h0 u1 < prime  /\ as_nat h0 u2 < prime  /\ as_nat h0 s1 < prime /\ as_nat h0 s2 < prime /\ as_nat h0 r < prime /\
+    as_nat h0 h < prime /\ as_nat h0 uh < prime /\ as_nat h0 hCube < prime /\
+    
+    eq_or_disjoint p result /\
+    LowStar.Monotonic.Buffer.all_disjoint [loc p; loc q; loc u1; loc u2; loc s1; loc s2; loc r; loc h; loc uh; loc hCube; loc tempBuffer28] /\ 
+    disjoint result tempBuffer28 /\
+    
+    as_nat h0 (gsub p (size 8) (size 4)) < prime /\ 
+    as_nat h0 (gsub p (size 0) (size 4)) < prime /\ 
+    as_nat h0 (gsub p (size 4) (size 4)) < prime /\ 
+    as_nat h0 (gsub q (size 0) (size 4)) < prime /\  
+    as_nat h0 (gsub q (size 4) (size 4)) < prime /\
+    
+    (
+      let pX, pY, pZ = as_nat h0 (gsub p (size 0) (size 4)), as_nat h0 (gsub p (size 4) (size 4)), as_nat h0 (gsub p (size 8) (size 4)) in 
+      let qX, qY, qZ = as_nat h0 (gsub q (size 0) (size 4)), as_nat h0 (gsub q (size 4) (size 4)), 1 in 
+      let pxD, pyD, pzD = fromDomain_ pX, fromDomain_ pY, fromDomain_ pZ in 
+      let qxD, qyD, qzD = fromDomain_ qX, fromDomain_ qY, fromDomain_ qZ in 
+
+      let u1D = fromDomain_ (as_nat h0 u1) in 
+      let u2D = fromDomain_ (as_nat h0 u2) in 
+      let s1D = fromDomain_ (as_nat h0 s1) in 
+      let s2D = fromDomain_ (as_nat h0 s2) in 
+
+      let hD = fromDomain_ (as_nat h0 h) in 
+      
+      as_nat h0 u1 == toDomain_ (qzD * qzD * pxD % prime256) /\
+      as_nat h0 u2 == toDomain_ (pzD * pzD * qxD % prime256) /\
+      as_nat h0 s1 == toDomain_ (qzD * qzD * qzD * pyD % prime256) /\
+      as_nat h0 s2 == toDomain_ (pzD * pzD * pzD * qyD % prime256) /\
+      
+      as_nat h0 h == toDomain_ ((u2D - u1D) % prime256) /\
+      as_nat h0 r == toDomain_ ((s2D - s1D) % prime256) /\
+      as_nat h0 uh == toDomain_ (hD * hD * u1D % prime256) /\
+      as_nat h0 hCube == toDomain_ (hD * hD * hD % prime256) 
+  )
+)
+  (ensures fun h0 _ h1 -> modifies (loc tempBuffer28 |+| loc result) h0 h1 /\
+    as_nat h1 (gsub result (size 8) (size 4)) < prime /\ 
+    as_nat h1 (gsub result (size 0) (size 4)) < prime /\  
+    as_nat h1 (gsub result (size 4) (size 4)) < prime /\
+    (
+      let pX, pY, pZ = as_nat h0 (gsub p (size 0) (size 4)), as_nat h0 (gsub p (size 4) (size 4)), as_nat h0 (gsub p (size 8) (size 4)) in 
+      let qX, qY, qZ = as_nat h0 (gsub q (size 0) (size 4)), as_nat h0 (gsub q (size 4) (size 4)), 1 in 
+      let x3, y3, z3 = as_nat h1 (gsub result (size 0) (size 4)), as_nat h1 (gsub result (size 4) (size 4)), as_nat h1 (gsub result (size 8) (size 4)) in  
+
+      let pxD, pyD, pzD = fromDomain_ pX, fromDomain_ pY, fromDomain_ pZ in 
+      let qxD, qyD, qzD = fromDomain_ qX, fromDomain_ qY, fromDomain_ qZ in 
+      let x3D, y3D, z3D = fromDomain_ x3, fromDomain_ y3, fromDomain_ z3 in 
+
+      let rD = fromDomain_ (as_nat h0 r) in 
+      let hD = fromDomain_ (as_nat h0 h) in 
+      let s1D = fromDomain_ (as_nat h0 s1) in 
+      let u1D = fromDomain_ (as_nat h0 u1) in 
+
+  if qzD = 0 then 
+    x3D == pxD /\ y3D == pyD /\ z3D == pzD
+   else if pzD = 0 then 
+    x3D == qxD /\  y3D == qyD /\ z3D == qzD
+   else 
+    x3 == toDomain_ ((rD * rD - hD * hD * hD - 2 * hD * hD * u1D) % prime256) /\ 
+    y3 == toDomain_(((hD * hD * u1D - fromDomain_ (x3)) * rD - s1D * hD * hD * hD) % prime256) /\
+    z3 == toDomain_ (pzD * qzD * hD % prime256) 
+  )
+)
 
 
 val cmovznz: out: felem -> x: felem -> y: felem -> mask: uint64 -> Stack unit
@@ -138,19 +253,19 @@ let cmovznz out x y mask =
   cmovznz4_lemma mask (Seq.index y 3) (Seq.index x 3)
 
 
-(*cmovzv to neq -> change order of argument *)
-val cmovznz_one_mm: out: felem -> x: felem -> mask: uint64 -> Stack unit
-  (requires fun h -> as_nat h x < prime256 /\ live h out /\ live h x /\ (uint_v mask == 0 \/ uint_v mask = pow2 64 - 1))
-  (ensures fun h0 _ h1 -> modifies (loc out) h0 h1 /\
+val cmovznz_one_mm: out: felem -> mask: uint64 -> Stack unit
+  (requires fun h ->
+    as_nat h out < prime256 /\
+    live h out /\ (uint_v mask == 0 \/ uint_v mask = pow2 64 - 1))
+  (ensures fun h0 _ h1 -> modifies (loc out) h0 h1 /\ 
     as_nat h1 out < prime256 /\ (
-    if v mask = 0
-      then as_nat h1 out == Spec.P256.MontgomeryMultiplication.toDomain_ 1 
-      else 
-	as_nat h1 out ==  as_nat h0 x ))
+    if v mask = 0 then 
+      as_nat h1 out == as_nat h0 out 
+    else 
+      as_nat h1 out ==  Spec.P256.MontgomeryMultiplication.toDomain_ 1))
 
-let cmovznz_one_mm out y mask = 
-  let h0 = ST.get() in 
-  
+let cmovznz_one_mm out mask = 
+
   let out_0 = index out (size 0) in 
   let out_1 = index out (size 1) in 
   let out_2 = index out (size 2) in 
@@ -160,39 +275,43 @@ let cmovznz_one_mm out y mask =
   let x_1 = u64 18446744069414584320 in 
   let x_2 = u64 18446744073709551615 in 
   let x_3 = u64 4294967294 in 
+  
+  let r_0 = logxor out_0 (logand mask (logxor out_0 x_0)) in 
+  let r_1 = logxor out_1 (logand mask (logxor out_1 x_1)) in 
+  let r_2 = logxor out_2 (logand mask (logxor out_2 x_2)) in 
+  let r_3 = logxor out_3 (logand mask (logxor out_3 x_3)) in 
 
-  let mask = eq_mask mask (u64 0) in 
-  let r0 = logor (logand x_0 mask) (logand y.(size 0) (lognot mask)) in 
-  let r1 = logor (logand x_1 mask) (logand y.(size 1) (lognot mask)) in 
-  let r2 = logor (logand x_2 mask) (logand y.(size 2) (lognot mask)) in 
-  let r3 = logor (logand x_3 mask) (logand y.(size 3) (lognot mask)) in 
+  lemma_xor_copy_cond out_0 x_0 mask;
+  lemma_xor_copy_cond out_1 x_1 mask;
+  lemma_xor_copy_cond out_2 x_2 mask;
+  lemma_xor_copy_cond out_3 x_3 mask;
 
-  upd out (size 0) r0;
-  upd out (size 1) r1;
-  upd out (size 2) r2;
-  upd out (size 3) r3;
+  upd out (size 0) r_0;
+  upd out (size 1) r_1;
+  upd out (size 2) r_2;
+  upd out (size 3) r_3;
+
 
   Spec.P256.MontgomeryMultiplication.lemmaToDomain 1;
   assert_norm(pow2 256 % prime256 = uint_v x_0 + uint_v x_1 * pow2 64 + uint_v x_2 * pow2 128 + uint_v x_3 * pow2 192);
   assert_norm (pow2 64 * pow2 64 = pow2 128);
-  assert_norm (pow2 64 * pow2 64 * pow2 64 = pow2 192);
-  
-  let y = as_seq h0 y in 
-  cmovznz4_lemma mask (Seq.index y 0) x_0;
-  cmovznz4_lemma mask (Seq.index y 1) x_1;
-  cmovznz4_lemma mask (Seq.index y 2) x_2;
-  cmovznz4_lemma mask (Seq.index y 3) x_3
+  assert_norm (pow2 64 * pow2 64 * pow2 64 = pow2 192)
 
 
-val copy_point_conditional: out: point -> p: point -> q: pointAffine -> maskPoint: point -> Stack unit 
-  (requires fun h -> live h out /\ live h p /\ live h q /\ live h maskPoint /\ disjoint p out /\ eq_or_disjoint q out /\
+val copy_point_conditional_affine_to_result: out: point 
+  -> q: pointAffine 
+  -> maskPoint: point
+  -> Stack unit 
+  (requires fun h -> live h out /\ live h q /\ live h maskPoint /\ disjoint q out /\ eq_or_disjoint out maskPoint /\
     (
-      let pX = as_nat h (gsub p (size 0) (size 4)) in 
-      let pY = as_nat h (gsub p (size 4) (size 4)) in 
-      let pZ = as_nat h (gsub p (size 8) (size 4)) in 
-      pX < prime256 /\ pY < prime256 /\ pZ < prime256 /\
       as_nat h (gsub q (size 0) (size 4)) < prime256 /\ 
-      as_nat h (gsub q (size 4) (size 4)) < prime256 
+      as_nat h (gsub q (size 4) (size 4)) < prime256 /\
+    
+      as_nat h (gsub out (size 0) (size 4)) < prime256 /\ 
+      as_nat h (gsub out (size 4) (size 4)) < prime256 /\
+      as_nat h (gsub out (size 8) (size 4)) < prime256 /\
+
+      as_nat h (gsub maskPoint (size 8) (size 4)) < prime256
     )
   )
   (ensures fun h0 _ h1 -> modifies (loc out) h0 h1 /\ (
@@ -201,495 +320,312 @@ val copy_point_conditional: out: point -> p: point -> q: pointAffine -> maskPoin
     let zOut = gsub out (size 8) (size 4) in 
     as_nat h1 xOut < prime256 /\
     as_nat h1 yOut < prime256 /\
-    as_nat h1 zOut < prime256 /\ (
-    
-    let mask = as_nat h0 (gsub maskPoint (size 8) (size 4)) in 
-    let xP = gsub p (size 0) (size 4) in 
-    let yP = gsub p (size 4) (size 4) in 
-    let zP = gsub p (size 8) (size 4) in 
+    as_nat h1 zOut < prime256  /\ (
+
+
+    let maskX = fromDomain_ (as_nat h0 (gsub maskPoint (size 0) (size 4))) in 
+    let maskY = fromDomain_ (as_nat h0 (gsub maskPoint (size 4) (size 4))) in 
+    let maskZ = fromDomain_ (as_nat h0 (gsub maskPoint (size 8) (size 4))) in 
 
     let xQ = gsub q (size 0) (size 4) in 
     let yQ = gsub q (size 4) (size 4) in 
 
-    if mask = 0 then 
+    if isPointAtInfinity (maskX, maskY, maskZ)  then 
       as_nat h1 xOut == as_nat h0 xQ /\ 
       as_nat h1 yOut == as_nat h0 yQ /\ 
-      as_nat h1 zOut == Spec.P256.MontgomeryMultiplication.toDomain_ 1
+      as_nat h1 zOut == Spec.P256.MontgomeryMultiplication.toDomain_ 1 
     else
-      as_nat h1 xOut == as_nat h0 xP /\ 
-      as_nat h1 yOut == as_nat h0 yP  /\ 
-      as_nat h1 zOut == as_nat h0 zP
-   
-     
-    ))) 
+      as_nat h1 xOut == as_nat h0 xOut /\ 
+      as_nat h1 yOut == as_nat h0 yOut /\ 
+      as_nat h1 zOut == as_nat h0 zOut)))
 
-let copy_point_conditional out p q maskPoint = 
-  let z = sub maskPoint (size 8) (size 4) in 
-  let mask = lognot (isZero_uint64_CT z) in 
-    lognot_lemma (isZero_uint64_CT z);
+
+let copy_point_conditional_affine_to_result out q maskPoint = 
+  let h0 = ST.get() in 
+  
+  let pZ = sub maskPoint (size 8) (size 4) in 
+  let mask = isZero_uint64_CT pZ in 
+
+  let xOut = sub out (size 0) (size 4) in 
+  let yOut = sub out (size 4) (size 4) in 
+  let zOut = sub out (size 8) (size 4) in 
+  
+  let qX = sub q (size 0) (size 4) in 
+  let qY = sub q (size 4) (size 4) in 
+
+  Hacl.Impl.P256.Q.PrimitivesMasking.copy_conditional xOut qX mask;
+  Hacl.Impl.P256.Q.PrimitivesMasking.copy_conditional yOut qY mask;
+  cmovznz_one_mm zOut mask;
+
+
+  lemma_multiplication_not_mod_prime (as_nat h0 pZ);
+  lemmaFromDomain (as_nat h0 pZ)
+
+
+val copy_point_conditional_jac_to_result: out: point 
+  -> q: point 
+  -> maskPoint: pointAffine
+  -> Stack unit 
+  (requires fun h -> live h out /\ live h q /\  eq_or_disjoint q out /\    
+    live h maskPoint /\ 
+    as_nat h (gsub q (size 0) (size 4)) < prime256 /\ 
+    as_nat h (gsub q (size 4) (size 4)) < prime256 /\
+    as_nat h (gsub q (size 8) (size 4)) < prime256 /\
+
+    as_nat h (gsub maskPoint (size 0) (size 4)) < prime256 /\
+    as_nat h (gsub maskPoint (size 4) (size 4)) < prime256 /\
+    
+    as_nat h (gsub out (size 0) (size 4)) < prime256 /\
+    as_nat h (gsub out (size 4) (size 4)) < prime256 /\
+    as_nat h (gsub out (size 8) (size 4)) < prime256)
+    
+  (ensures fun h0 _ h1 -> modifies (loc out) h0 h1 /\ (
+    let xOut = gsub out (size 0) (size 4) in 
+    let yOut = gsub out (size 4) (size 4) in 
+    let zOut = gsub out (size 8) (size 4) in 
+    as_nat h1 xOut < prime256 /\
+    as_nat h1 yOut < prime256 /\
+    as_nat h1 zOut < prime256 /\ (
+
+    let xQ = gsub q (size 0) (size 4) in 
+    let yQ = gsub q (size 4) (size 4) in 
+    let zQ = gsub q (size 8) (size 4) in 
+
+    if isPointAtInfinityAffine (
+      as_nat h0 (gsub maskPoint (size 0) (size 4)), 
+      as_nat h0 (gsub maskPoint (size 4) (size 4)))
+    then    
+          as_nat h1 xOut == as_nat h0 xQ /\ 
+      as_nat h1 yOut == as_nat h0 yQ /\ 
+      as_nat h1 zOut == as_nat h0 zQ
+    else
+
+      as_nat h1 xOut == as_nat h0 xOut /\ 
+      as_nat h1 yOut == as_nat h0 yOut /\ 
+      as_nat h1 zOut == as_nat h0 zOut
+      
+      )))
+
+
+let copy_point_conditional_jac_to_result out q maskPoint = 
+  
+  let mask = pointAffineIsNotZero maskPoint in 
 
   let xOut = sub out (size 0) (size 4) in 
   let yOut = sub out (size 4) (size 4) in 
   let zOut = sub out (size 8) (size 4) in 
 
-  let pX = sub p (size 0) (size 4) in 
-  let pY = sub p (size 4) (size 4) in 
-  let pZ = sub p (size 8) (size 4) in 
-
   let qX = sub q (size 0) (size 4) in 
   let qY = sub q (size 4) (size 4) in 
+  let qZ = sub q (size 8) (size 4) in 
 
-  cmovznz4 mask qX pX xOut;
-  cmovznz4 mask qY pY yOut;
-  cmovznz_one_mm zOut pZ mask 
-
-
-let prime = prime256 
-
-val point_add_step0: result: point -> p: point -> q: pointAffine -> tempBuffer: lbuffer uint64 (size 20) -> Stack unit
-  (requires fun h -> live h result /\ live h p /\ live h q /\ live h tempBuffer /\
-    disjoint p tempBuffer /\ disjoint q tempBuffer /\ (
-    let x1 = gsub p (size 0) (size 4) in 
-    let y1 = gsub p (size 4) (size 4) in 
-    let z1 = gsub p (size 8) (size 4) in 
-
-    let x2 = gsub q (size 0) (size 4) in 
-    let y2 = gsub q (size 4) (size 4) in 
-
-    as_nat h x1 < prime256 /\
-    as_nat h y1 < prime256 /\
-    as_nat h z1 < prime256 /\
-
-    as_nat h x2 < prime256 /\
-    as_nat h y2 < prime256 ))
-  (ensures fun h0 _ h1 -> modifies (loc tempBuffer) h0 h1 /\ (
-    let x1D = fromDomain_ (as_nat h0 (gsub p (size 0) (size 4))) in 
-    let x2D = fromDomain_ (as_nat h0 (gsub q (size 0) (size 4))) in 
-    let y1D = fromDomain_ (as_nat h0 (gsub p (size 4) (size 4))) in 
-    let y2D = fromDomain_ (as_nat h0 (gsub q (size 4) (size 4))) in 
-    let z1D = fromDomain_ (as_nat h0 (gsub p (size 8) (size 4))) in 
-
-    let t0 = gsub tempBuffer (size 0) (size 4) in 
-    let t1 = gsub tempBuffer (size 4) (size 4) in 
-    let t3 = gsub tempBuffer (size 12) (size 4) in 
-    let t4 = gsub tempBuffer (size 16) (size 4) in 
-
-    let t0_ = (x1D * x2D) % prime in 
-    let t1_ = (y1D * y2D) % prime in 
-    let t3_ = (x2D + y2D) % prime in 
-    let t4_ = (x1D + y1D) % prime in 
-
-    let t3_ = (t3_ * t4_) % prime in 
-    let t4_ = (t0_ + t1_) % prime in 
-    let t3_ = (t3_ - t4_) % prime in 
-    let t4_ = (y2D - z1D) % prime in 
-    
-    as_nat h1 t0 = toDomain_ t0_ /\
-    as_nat h1 t1 = toDomain_ t1_ /\
-    as_nat h1 t3 = toDomain_ t3_ /\
-    as_nat h1 t4 = toDomain_ t4_ /\
-    
-    as_nat h1 t0 < prime /\
-    as_nat h1 t1 < prime /\
-    as_nat h1 t3 < prime /\
-    as_nat h1 t4 < prime))
+  Hacl.Impl.P256.Q.PrimitivesMasking.copy_conditional xOut qX mask;
+  Hacl.Impl.P256.Q.PrimitivesMasking.copy_conditional yOut qY mask;
+  Hacl.Impl.P256.Q.PrimitivesMasking.copy_conditional zOut qZ mask
 
 
-let point_add_step0 result p q tempBuffer = 
-  let x1 = sub p (size 0) (size 4) in 
-  let y1 = sub p (size 4) (size 4) in 
-  let z1 = sub p (size 8) (size 4) in 
+val copy_point_conditional: result: point -> x: point -> p: point -> maskPoint: pointAffine -> Stack unit
+  (requires fun h -> live h result /\ live h p /\ live h maskPoint /\ live h x /\
+    disjoint x result /\ eq_or_disjoint p result /\
+    as_nat h (gsub p (size 0) (size 4)) < prime /\ 
+    as_nat h (gsub p (size 4) (size 4)) < prime /\ 
+    as_nat h (gsub p (size 8) (size 4)) < prime /\
 
-  let x2 = sub q (size 0) (size 4) in 
-  let y2 = sub q (size 4) (size 4) in 
+    as_nat h (gsub x (size 0) (size 4)) < prime /\ 
+    as_nat h (gsub x (size 4) (size 4)) < prime /\ 
+    as_nat h (gsub x (size 8) (size 4)) < prime /\
 
-  let t0 = sub tempBuffer (size 0) (size 4) in 
-  let t1 = sub tempBuffer (size 4) (size 4) in 
-  let t3 = sub tempBuffer (size 12) (size 4) in 
-  let t4 = sub tempBuffer (size 16) (size 4) in 
-
-  montgomery_multiplication_buffer t0 x1 x2;
-  montgomery_multiplication_buffer t1 y1 y2;
-  p256_add t3 x2 y2;  
-  p256_add t4 x1 y1;
+    as_nat h (gsub maskPoint (size 0) (size 4)) < prime /\
+    as_nat h (gsub maskPoint (size 4) (size 4)) < prime)
+  (ensures fun h0 _ h1 -> modifies (loc result) h0 h1 /\
   
-  montgomery_multiplication_buffer t3 t3 t4;
-  p256_add t4 t0 t1;
-  p256_sub t3 t3 t4;
-  p256_sub t4 y2 z1
-
-
-val point_add_step1: result: point -> p: point -> q: pointAffine -> tempBuffer: lbuffer uint64 (size 20) -> Stack unit
-  (requires fun h -> live h result /\ live h p /\ live h q /\ live h tempBuffer /\
-    disjoint q result /\ disjoint p tempBuffer /\ disjoint q tempBuffer /\ eq_or_disjoint result p /\ disjoint result tempBuffer /\ (
-    let t1 = gsub tempBuffer (size 4) (size 4) in 
-    let t4 = gsub tempBuffer (size 16) (size 4) in  
-
-    let x1 = gsub p (size 0) (size 4) in 
-    let y1 = gsub p (size 4) (size 4) in 
-    let z1 = gsub p (size 8) (size 4) in 
-
-    let x2 = gsub q (size 0) (size 4) in 
-    let y2 = gsub q (size 4) (size 4) in 
-
-    as_nat h x1 < prime256 /\
-    as_nat h y1 < prime256 /\
-    as_nat h z1 < prime256 /\
-
-    as_nat h x2 < prime256 /\
-    as_nat h y2 < prime256 /\
-
-    as_nat h t1 < prime /\ 
-    as_nat h t4 < prime 
+  as_nat h1 (gsub result (size 0) (size 4)) < prime /\ 
+  as_nat h1 (gsub result (size 4) (size 4)) < prime /\ 
+  as_nat h1 (gsub result (size 8) (size 4)) < prime /\ (
   
-  ))
-  (ensures fun h0 _ h1 -> modifies (loc result |+| loc tempBuffer) h0 h1 /\ (
-    let x1D = fromDomain_ (as_nat h0 (gsub p (size 0) (size 4))) in 
-    let x2D = fromDomain_ (as_nat h0 (gsub q (size 0) (size 4))) in 
-    let y1D = fromDomain_ (as_nat h0 (gsub p (size 4) (size 4))) in 
-    let y2D = fromDomain_ (as_nat h0 (gsub q (size 4) (size 4))) in 
-    let z1D = fromDomain_ (as_nat h0 (gsub p (size 8) (size 4))) in 
+  if isPointAtInfinityAffine 
+    (fromDomain_ (as_nat h0 (gsub maskPoint (size 0) (size 4))), 
+    fromDomain_ (as_nat h0 (gsub maskPoint (size 4) (size 4))))
+  then 
+    as_nat h1 (gsub result (size 0) (size 4)) == as_nat h0 (gsub p (size 0) (size 4)) /\
+    as_nat h1 (gsub result (size 4) (size 4)) == as_nat h0 (gsub p (size 4) (size 4)) /\
+    as_nat h1 (gsub result (size 8) (size 4)) == as_nat h0 (gsub p (size 8) (size 4)) 
+  else
+    as_nat h1 (gsub result (size 0) (size 4)) == as_nat h0 (gsub x (size 0) (size 4)) /\
+    as_nat h1 (gsub result (size 4) (size 4)) == as_nat h0 (gsub x (size 4) (size 4)) /\
+    as_nat h1 (gsub result (size 8) (size 4)) == as_nat h0 (gsub x (size 8) (size 4))))
 
-    let x3 = gsub result (size 0) (size 4) in 
-    let y3 = gsub result (size 4) (size 4) in 
-    let z3 = gsub result (size 8) (size 4) in 
+let copy_point_conditional result x p maskPoint = 
+  let h0 = ST.get() in 
 
-    let t0 = gsub tempBuffer (size 0) (size 4) in 
-    let t1 = gsub tempBuffer (size 4) (size 4) in 
-    let t2 = gsub tempBuffer (size 8) (size 4) in 
-    let t3 = gsub tempBuffer (size 12) (size 4) in 
-    let t4 = gsub tempBuffer (size 16) (size 4) in 
+  let mask = pointAffineIsNotZero maskPoint in 
 
-    let t1D = fromDomain_ (as_nat h0 t1) in 
-    let t4D = fromDomain_ (as_nat h0 t4) in 
+  let p_x = sub p (size 0) (size 4) in 
+  let p_y = sub p (size 4) (size 4) in 
+  let p_z = sub p (size 8) (size 4) in 
 
-    let t4_ = (t4D + y1D) % prime in 
-    let y3_ = (x2D * z1D) % prime in
-    let y3_ = (y3_ + x1D) % prime in 
-    let z3_ = (Spec.P256.bCoordinateP256 * z1D) % prime in 
+  let x_x = sub x (size 0) (size 4) in 
+  let x_y = sub x (size 4) (size 4) in 
+  let x_z = sub x (size 8) (size 4) in 
 
-    let x3_ = (y3_ - z3_) % prime in 
-    let z3_ = (x3_ + x3_) % prime in 
-    let x3_ = (x3_ + z3_)  % prime in 
-    let z3_ = (t1D - x3_) % prime in 
-    let x3_ = (t1D + x3_) % prime in 
-    let y3_ = (Spec.P256.bCoordinateP256 * y3_) % prime in 
+  let result_x = sub result (size 0) (size 4) in 
+  let result_y = sub result (size 4) (size 4) in 
+  let result_z = sub result (size 8) (size 4) in 
 
-    as_nat h1 x3 = toDomain_ x3_ /\ 
-    as_nat h1 y3 = toDomain_ y3_ /\
-    as_nat h1 z3 = toDomain_ z3_ /\
+  cmovznz4 mask x_x p_x result_x;
+  cmovznz4 mask x_y p_y result_y;
+  cmovznz4 mask x_z p_z result_z;
 
-    as_nat h0 t0 = as_nat h1 t0 /\
-    as_nat h0 t1 = as_nat h1 t1 /\
-    as_nat h0 t3 = as_nat h1 t3 /\
-    as_nat h1 t4 = toDomain_ t4_ /\
+  let mX = as_nat h0 (gsub maskPoint (size 0) (size 4)) in 
+  let mY = as_nat h0 (gsub maskPoint (size 4) (size 4)) in 
 
-    as_nat h1 x3 < prime /\
-    as_nat h1 y3 < prime /\
-    as_nat h1 z3 < prime /\
+  lemma_multiplication_not_mod_prime mX;
+  lemmaFromDomain mX;
+
+  lemma_multiplication_not_mod_prime mY;
+  lemmaFromDomain mY
+
+
+inline_for_extraction noextract 
+val point_add_if_second_branch_impl_mixed: result: point -> p: point -> q: pointAffine 
+  -> u1: felem -> u2: felem -> s1: felem -> s2: felem -> r: felem -> h: felem -> uh: felem 
+  -> hCube: felem -> tempBuffer28 : lbuffer uint64 (size 28) -> 
+  Stack unit 
+    (requires fun h0 -> live h0 result /\ live h0 p /\ live h0 q /\ live h0 u1 /\ live h0 u2 /\ live h0 s1 /\ live h0 s2 /\ live h0 r /\ live h0 h /\ live h0 uh /\ live h0 hCube /\ live h0 tempBuffer28 /\
     
-    as_nat h1 t4 < prime ))
-
-let point_add_step1 result p q tempBuffer = 
-  let x1 = sub p (size 0) (size 4) in 
-  let y1 = sub p (size 4) (size 4) in 
-  let z1 = sub p (size 8) (size 4) in 
-
-  let x2 = sub q (size 0) (size 4) in 
-  let y2 = sub q (size 4) (size 4) in 
-
-  let t0 = sub tempBuffer (size 0) (size 4) in 
-  let t1 = sub tempBuffer (size 4) (size 4) in 
-  let t2 = sub tempBuffer (size 8) (size 4) in 
-  let t3 = sub tempBuffer (size 12) (size 4) in 
-  let t4 = sub tempBuffer (size 16) (size 4) in 
-
-  let x3 = sub result (size 0) (size 4) in 
-  let y3 = sub result (size 4) (size 4) in 
-  let z3 = sub result (size 8) (size 4) in 
-  Hacl.Impl.P256.LowLevel.PrimeSpecific.upload_p256_point_on_curve_constant t2;
-
-  p256_add t4 t4 y1; 
-  montgomery_multiplication_buffer y3 x2 z1; 
-  p256_add y3 y3 x1;
-  montgomery_multiplication_buffer z3 t2 z1; 
-
-  
-  p256_sub x3 y3 z3;
-  p256_add z3 x3 x3;
-  p256_add x3 x3 z3; 
-  p256_sub z3 t1 x3; 
-  p256_add x3 t1 x3; 
-  montgomery_multiplication_buffer y3 t2 y3
-
-
-val point_add_step2: result: point -> p: point -> q: pointAffine -> tempBuffer: lbuffer uint64 (size 20) -> Stack unit
-  (requires fun h -> live h result /\ live h p /\ live h q /\ live h tempBuffer /\
-    disjoint p tempBuffer /\ disjoint q tempBuffer /\ eq_or_disjoint result p /\ disjoint result tempBuffer /\ (
-    let t0 = gsub tempBuffer (size 0) (size 4) in 
-    let t1 = gsub tempBuffer (size 4) (size 4) in 
-    let t2 = gsub tempBuffer (size 8) (size 4) in 
-    let t4 = gsub tempBuffer (size 16) (size 4) in  
-
-    let x1 = gsub p (size 0) (size 4) in 
-    let y1 = gsub p (size 4) (size 4) in 
-    let z1 = gsub p (size 8) (size 4) in 
-
-    let x2 = gsub q (size 0) (size 4) in 
-    let y2 = gsub q (size 4) (size 4) in 
-
-    let x3 = gsub result (size 0) (size 4) in 
-    let y3 = gsub result (size 4) (size 4) in 
-    let z3 = gsub result (size 8) (size 4) in 
-
-    as_nat h x1 < prime256 /\
-    as_nat h y1 < prime256 /\
-    as_nat h z1 < prime256 /\
-
-    as_nat h x2 < prime256 /\
-    as_nat h y2 < prime256 /\
-
-    as_nat h x3 < prime256 /\
-    as_nat h y3 < prime256 /\
-    as_nat h z3 < prime256 /\
-
-    as_nat h t0 < prime /\
-    as_nat h t1 < prime /\ 
-    as_nat h t4 < prime))
-  (ensures fun h0 _ h1 -> modifies (loc result |+| loc tempBuffer) h0 h1 /\ (
-    let z1D = fromDomain_ (as_nat h0 (gsub p (size 8) (size 4))) in 
-    let y3D = fromDomain_ (as_nat h0 (gsub result (size 4) (size 4))) in 
-
-    let x3 = gsub result (size 0) (size 4) in 
-    let y3 = gsub result (size 4) (size 4) in 
-    let z3 = gsub result (size 8) (size 4) in 
-
-    let t0 = gsub tempBuffer (size 0) (size 4) in 
-    let t1 = gsub tempBuffer (size 4) (size 4) in 
-    let t2 = gsub tempBuffer (size 8) (size 4) in 
-    let t3 = gsub tempBuffer (size 12) (size 4) in 
-    let t4 = gsub tempBuffer (size 16) (size 4) in 
-
-    let t0D = fromDomain_ (as_nat h0 t0) in 
-    let t4D = fromDomain_ (as_nat h0 t4) in 
-
-    let t1_ = (z1D + z1D) % prime in 
-    let t2_ = (t1_ + z1D) % prime in 
-    let y3_ = (y3D - t2_) % prime in 
-    let y3_ = (y3_ - t0D) % prime in 
-    let t1_ = (y3_ + y3_) % prime in 
-
-    let y3_ = (t1_ + y3_) % prime in 
-    let t1_ = (t0D + t0D) % prime in 
-    let t0_ = (t1_ + t0D) % prime in 
-    let t0_ = (t0_ - t2_) % prime in 
-    let t1_ = (t4D * y3_) % prime in 
-
-    as_nat h1 t0 = toDomain_ t0_ /\
-    as_nat h1 t1 = toDomain_ t1_ /\
-    as_nat h1 t2 = toDomain_ t2_ /\
-    as_nat h1 t3 = as_nat h0 t3 /\
-    as_nat h1 t4 = as_nat h0 t4 /\
-
-    as_nat h1 x3 = as_nat h0 x3 /\
-    as_nat h1 y3 = toDomain_ y3_ /\
-    as_nat h1 z3 = as_nat h0 z3 /\
-
-    as_nat h1 t0 < prime /\
-    as_nat h1 t1 < prime /\
-    as_nat h1 t2 < prime /\
-
-    as_nat h1 y3 < prime))
-
-
-let point_add_step2 result p q tempBuffer = 
-  let x1 = sub p (size 0) (size 4) in 
-  let y1 = sub p (size 4) (size 4) in 
-  let z1 = sub p (size 8) (size 4) in 
-
-  let x2 = sub q (size 0) (size 4) in 
-  let y2 = sub q (size 4) (size 4) in 
-
-  let t0 = sub tempBuffer (size 0) (size 4) in 
-  let t1 = sub tempBuffer (size 4) (size 4) in 
-  let t2 = sub tempBuffer (size 8) (size 4) in 
-  let t3 = sub tempBuffer (size 12) (size 4) in 
-  let t4 = sub tempBuffer (size 16) (size 4) in 
-
-  let x3 = sub result (size 0) (size 4) in 
-  let y3 = sub result (size 4) (size 4) in 
-  let z3 = sub result (size 8) (size 4) in 
-
-  p256_add t1 z1 z1;
-  p256_add t2 t1 z1;
-  p256_sub y3 y3 t2;
-  p256_sub y3 y3 t0;
-  p256_add t1 y3 y3;
-
-  p256_add y3 t1 y3;
-  p256_add t1 t0 t0;
-  p256_add t0 t1 t0;
-  p256_sub t0 t0 t2;
-  montgomery_multiplication_buffer t1 t4 y3
-
-
-val point_add_step3: result: point -> p: point -> q: pointAffine -> tempBuffer: lbuffer uint64 (size 20) -> Stack unit
-  (requires fun h -> live h result /\ live h p /\ live h q /\ live h tempBuffer /\
-    disjoint p tempBuffer /\ disjoint q tempBuffer /\ eq_or_disjoint result p /\ disjoint result tempBuffer /\ (
-    let t0 = gsub tempBuffer (size 0) (size 4) in 
-    let t1 = gsub tempBuffer (size 4) (size 4) in 
-    let t2 = gsub tempBuffer (size 8) (size 4) in 
-    let t3 = gsub tempBuffer (size 12) (size 4) in 
-    let t4 = gsub tempBuffer (size 16) (size 4) in  
-
-    let x1 = gsub p (size 0) (size 4) in 
-    let y1 = gsub p (size 4) (size 4) in 
-    let z1 = gsub p (size 8) (size 4) in 
-
-    let x2 = gsub q (size 0) (size 4) in 
-    let y2 = gsub q (size 4) (size 4) in 
-
-    let x3 = gsub result (size 0) (size 4) in 
-    let y3 = gsub result (size 4) (size 4) in 
-    let z3 = gsub result (size 8) (size 4) in 
-
-    as_nat h x1 < prime256 /\
-    as_nat h y1 < prime256 /\
-    as_nat h z1 < prime256 /\
-
-    as_nat h x2 < prime256 /\
-    as_nat h y2 < prime256 /\
-
-    as_nat h x3 < prime256 /\
-    as_nat h y3 < prime256 /\
-    as_nat h z3 < prime256 /\
-
-    as_nat h t0 < prime /\
-    as_nat h t1 < prime /\ 
-    as_nat h t2 < prime /\
-    as_nat h t3 < prime /\
-    as_nat h t4 < prime))
-  (ensures fun h0 _ h1 -> modifies (loc result |+| loc tempBuffer) h0 h1 /\ (
-    let x3 = gsub result (size 0) (size 4) in 
-    let y3 = gsub result (size 4) (size 4) in 
-    let z3 = gsub result (size 8) (size 4) in 
-
-    let x3D = fromDomain_ (as_nat h0 x3) in 
-    let y3D = fromDomain_ (as_nat h0 y3) in 
-    let z3D = fromDomain_ (as_nat h0 z3) in 
-
-    let t0 = gsub tempBuffer (size 0) (size 4) in 
-    let t1 = gsub tempBuffer (size 4) (size 4) in 
-    let t2 = gsub tempBuffer (size 8) (size 4) in 
-    let t3 = gsub tempBuffer (size 12) (size 4) in 
-    let t4 = gsub tempBuffer (size 16) (size 4) in   
-
-    let t0D = fromDomain_ (as_nat h0 t0) in 
-    let t1D = fromDomain_ (as_nat h0 t1) in 
-    let t3D = fromDomain_ (as_nat h0 t3) in 
-    let t4D = fromDomain_ (as_nat h0 t4) in 
+    as_nat h0 u1 < prime /\ as_nat h0 u2 < prime /\ as_nat h0 s1 < prime /\ as_nat h0 s2 < prime /\
+    as_nat h0 r < prime /\ as_nat h0 h < prime /\ as_nat h0 uh < prime /\ as_nat h0 hCube < prime /\
     
+    eq_or_disjoint result p /\
+    LowStar.Monotonic.Buffer.all_disjoint [loc result; loc q; loc hCube; loc uh; loc r; loc tempBuffer28; loc s1; loc h] /\
+    disjoint p tempBuffer28 /\
 
-    let t2_ = (t0D * y3D) % prime in
-    let y3_ = (x3D * z3D) % prime in 
-    let y3_ = (y3_ + t2_) % prime in 
-    let x3_ = (t3D * x3D) % prime in 
+    as_nat h0 (gsub p (size 8) (size 4)) < prime /\ 
+    as_nat h0 (gsub p (size 0) (size 4)) < prime /\ 
+    as_nat h0 (gsub p (size 4) (size 4)) < prime /\
+    as_nat h0 (gsub q (size 0) (size 4)) < prime /\  
+    as_nat h0 (gsub q (size 4) (size 4)) < prime /\ (
 
-    let x3_ = (x3_ - t1D) % prime in 
-    let z3_ = (t4D * z3D) % prime in 
-    let t1_ = (t3D * t0D) % prime in 
-    let z3_ = (z3_ * t1_) % prime in 
+    let pX, pY, pZ = as_nat h0 (gsub p (size 0) (size 4)), as_nat h0 (gsub p (size 4) (size 4)), as_nat h0 (gsub p (size 8) (size 4)) in 
+    let qX, qY, qZ = as_nat h0 (gsub q (size 0) (size 4)), as_nat h0 (gsub q (size 4) (size 4)), 1 in 
+    let pxD, pyD, pzD = fromDomain_ pX, fromDomain_ pY, fromDomain_ pZ in 
+    let qxD, qyD, qzD = fromDomain_ qX, fromDomain_ qY, fromDomain_ qZ in 
 
-    as_nat h1 t1 = toDomain_ t1_ /\
-    as_nat h1 t2 = toDomain_ t2_ /\
-   
-    as_nat h1 x3 = toDomain_ x3_ /\ 
-    as_nat h1 y3 = toDomain_ y3_ /\
-    as_nat h1 z3 = toDomain_ z3_ /\
+    let u1D = fromDomain_ (as_nat h0 u1) in 
+    let u2D = fromDomain_ (as_nat h0 u2) in 
+    let s1D = fromDomain_ (as_nat h0 s1) in 
+    let s2D = fromDomain_ (as_nat h0 s2) in 
 
-    as_nat h1 x3 < prime /\
-    as_nat h1 y3 < prime /\
-    as_nat h1 z3 < prime ))
-
-
-let point_add_step3 result p q tempBuffer = 
-  let x1 = sub p (size 0) (size 4) in 
-  let y1 = sub p (size 4) (size 4) in 
-  let z1 = sub p (size 8) (size 4) in 
-
-  let x2 = sub q (size 0) (size 4) in 
-  let y2 = sub q (size 4) (size 4) in 
-
-  let t0 = sub tempBuffer (size 0) (size 4) in 
-  let t1 = sub tempBuffer (size 4) (size 4) in 
-  let t2 = sub tempBuffer (size 8) (size 4) in 
-  let t3 = sub tempBuffer (size 12) (size 4) in 
-  let t4 = sub tempBuffer (size 16) (size 4) in 
-
-  let x3 = sub result (size 0) (size 4) in 
-  let y3 = sub result (size 4) (size 4) in 
-  let z3 = sub result (size 8) (size 4) in 
-
-  montgomery_multiplication_buffer t2 t0 y3;
-  montgomery_multiplication_buffer y3 x3 z3;
-  p256_add y3 y3 t2;
-  montgomery_multiplication_buffer x3 t3 x3;
-
-  p256_sub x3 x3 t1;
-  montgomery_multiplication_buffer z3 t4 z3;
-  montgomery_multiplication_buffer t1 t3 t0;
-  montgomery_multiplication_buffer z3 z3 t1
-
-
-#push-options "--z3rlimit 300"
-
-(* we expect that we already know the q point *)
-(* Change the size f byffer *)
-val pointAddMixed: result: point -> p: point -> q: pointAffine -> tempBuffer: lbuffer uint64 (size 100) -> Stack unit 
-  (requires fun h -> live h result /\ live h p /\ live h q /\ disjoint q result /\ disjoint result p /\ (
-    let x1 = gsub p (size 0) (size 4) in 
-    let y1 = gsub p (size 4) (size 4) in 
-    let z1 = gsub p (size 8) (size 4) in 
-
-    let x2 = gsub q (size 0) (size 4) in 
-    let y2 = gsub q (size 4) (size 4) in 
-
-    as_nat h x1 < prime256 /\
-    as_nat h y1 < prime256 /\
-    as_nat h z1 < prime256 /\
-
-    as_nat h x2 < prime256 /\
-    as_nat h y2 < prime256)
-  )
-  (ensures fun h0 _ h1 -> modifies (loc result) h0 h1 /\    
+    let hD = fromDomain_ (as_nat h0 h) in 
+      
+    as_nat h0 u1 == toDomain_ (pxD % prime256) /\
+    as_nat h0 u2 == toDomain_ (pzD * pzD * qxD % prime256) /\
+    as_nat h0 s1 == toDomain_ (pyD % prime256) /\
+    as_nat h0 s2 == toDomain_ (pzD * pzD * pzD * qyD % prime256) /\
+      
+    as_nat h0 h == toDomain_ ((u2D - u1D) % prime256) /\
+    as_nat h0 r == toDomain_ ((s2D - s1D) % prime256) /\
+    as_nat h0 uh == toDomain_ (hD * hD * u1D % prime256) /\
+    as_nat h0 hCube == toDomain_ (hD * hD * hD % prime256)))
+  (ensures fun h0 _ h1 -> modifies (loc tempBuffer28 |+| loc result) h0 h1 /\
     as_nat h1 (gsub result (size 8) (size 4)) < prime /\ 
-    as_nat h1 (gsub result (size 0) (size 4)) < prime /\ 
+    as_nat h1 (gsub result (size 0) (size 4)) < prime /\  
     as_nat h1 (gsub result (size 4) (size 4)) < prime /\ (
     
-    let pX, pY, pZ = gsub p (size 0) (size 4), gsub p (size 4) (size 4), gsub p (size 8) (size 4) in 
-    let qX, qY = gsub q (size 0) (size 4), gsub q (size 4) (size 4) in 
-    let x3, y3, z3 = gsub result (size 0) (size 4), gsub result (size 4) (size 4), gsub result (size 8) (size 4) in 
-       
-    let pxD, pyD, pzD = fromDomain_ (as_nat h0 pX), fromDomain_ (as_nat h0 pY), fromDomain_ (as_nat h0 pZ) in 
-    let qxD, qyD = fromDomain_ (as_nat h0 qX), fromDomain_ (as_nat h0 qY) in 
-    let x3D, y3D, z3D = fromDomain_ (as_nat h1 x3), fromDomain_ (as_nat h1 y3), fromDomain_ (as_nat h1 z3) in
-      
-    let xN, yN, zN = Spec.P256.point_add_mixed (pxD, pyD, pzD) (qxD, qyD) in 
-    x3D == xN /\ y3D == yN /\ z3D == zN))
+    let pX, pY, pZ = as_nat h0 (gsub p (size 0) (size 4)), as_nat h0 (gsub p (size 4) (size 4)), as_nat h0 (gsub p (size 8) (size 4)) in 
+    let qX, qY, qZ = as_nat h0 (gsub q (size 0) (size 4)), as_nat h0 (gsub q (size 4) (size 4)), toDomain_ 1 in 
+    let x3, y3, z3 = as_nat h1 (gsub result (size 0) (size 4)), as_nat h1 (gsub result (size 4) (size 4)), as_nat h1 (gsub result (size 8) (size 4)) in  
+
+    let pxD, pyD, pzD = fromDomain_ pX, fromDomain_ pY, fromDomain_ pZ in 
+    let qxD, qyD, qzD = fromDomain_ qX, fromDomain_ qY, fromDomain_ qZ in 
+    let x3D, y3D, z3D = fromDomain_ x3, fromDomain_ y3, fromDomain_ z3 in 
+
+    let rD = fromDomain_ (as_nat h0 r) in 
+    let hD = fromDomain_ (as_nat h0 h) in 
+    let s1D = fromDomain_ (as_nat h0 s1) in 
+    let u1D = fromDomain_ (as_nat h0 u1) in 
+    
+    if isPointAtInfinityAffine  (qxD, qyD) then 
+      x3D == pxD /\ y3D == pyD /\ z3D == pzD
+    else if isPointAtInfinity (pxD, pyD, pzD) then 
+      x3D == qxD /\  y3D == qyD /\ z3D == 1 
+    else 
+      x3 == toDomain_ ((rD * rD - hD * hD * hD - 2 * hD * hD * u1D) % prime256) /\ 
+      y3 == toDomain_(((hD * hD * u1D - fromDomain_ x3) * rD - s1D * hD * hD * hD) % prime256) /\
+      z3 == toDomain_ (pzD * hD % prime256)))
 
 
-let pointAddMixed result p q tempBuffer = 
-  push_frame();
-    let tempBuffer = sub tempBuffer (size 0) (u64 20) in 
-    let tempPoint = sub tempBuffer (size 20) (u64 12) in 
-      let h0 = ST.get() in 
-    point_add_step0 tempPoint p q tempBuffer; 
-    point_add_step1 tempPoint p q tempBuffer; 
-    point_add_step2 tempPoint p q tempBuffer; 
-    point_add_step3 tempPoint p q tempBuffer; 
-    copy_point_conditional result tempPoint q p;
-    Hacl.Impl.P256.Math.lemma_multiplication_not_mod_prime (as_nat h0 (gsub p (size 8) (size 4)));
-    lemmaFromDomain (as_nat h0 (gsub p (size 8) (size 4)));
-  pop_frame()
+let point_add_if_second_branch_impl_mixed result p q u1 u2 s1 s2 r h uh hCube tempBuffer28 = 
+    let h0 = ST.get() in 
+  let pZ = sub p (size 8) (size 4) in
 
-#pop-options
+  let tempBuffer16 = sub tempBuffer28 (size 0) (size 16) in 
+
+
+  let pointOut = Lib.Buffer.sub tempBuffer28 (size 16) (size 12) in 
+  let xOut = Lib.Buffer.sub tempBuffer28 (size 16) (size 4) in 
+  let yOut = Lib.Buffer.sub tempBuffer28 (size 20) (size 4) in 
+  let zOut = Lib.Buffer.sub tempBuffer28 (size 24) (size 4) in 
+
+
+  Hacl.Impl.P256.PointAdd.computeX3_point_add xOut hCube uh r tempBuffer16; 
+  Hacl.Impl.P256.PointAdd.computeY3_point_add yOut s1 hCube uh xOut r tempBuffer16;
+
+    let h1 = ST.get() in 
+
+  computeZ3_point_add_mixed zOut pZ h;
+  copy_point_conditional_affine_to_result pointOut q p; 
+  copy_point_conditional result pointOut p q; 
+
+  let rD = fromDomain_ (as_nat h0 r) in 
+  let hD = fromDomain_ (as_nat h0 h) in
+  let u1D = fromDomain_ (as_nat h0 u1) in 
+  let uhD = fromDomain_ (as_nat h0 uh) in 
+
+  let s1D = fromDomain_ (as_nat h0 s1) in 
+  let x3D = fromDomain_ (as_nat h1 xOut) in 
+
+
+  lemma_point_add_0 (rD * rD) (hD * hD * hD) (hD * hD * u1D);
+  lemma_mod_sub_distr (rD * rD - 2 * uhD) (hD * hD * hD) prime256;
+  assert_by_tactic (2 * (hD * hD * u1D) == 2 * hD * hD * u1D) canon;
+
+  lemma_point_add_1 (hD * hD * u1D) x3D rD s1D (hD * hD * hD);
+  assert_by_tactic (s1D * (hD * hD * hD) == s1D * hD * hD * hD) canon;
+
+  assert_norm (modp_inv2 (pow2 256) > 0);
+  assert_norm (modp_inv2 (pow2 256) % prime <> 0)
+
+
+let point_add_mixed p q result tempBuffer = 
+    let h0 = ST.get() in 
+  
+  let tempBuffer28 = sub tempBuffer (size 0) (size 28) in 
+  let tempBuffer16 = sub tempBuffer (size 0) (size 16) in 
+   
+  let u1 = sub tempBuffer (size 28) (size 4) in 
+  let u2 = sub tempBuffer (size 32) (size 4) in 
+  let s1 = sub tempBuffer (size 36) (size 4) in 
+  let s2 = sub tempBuffer (size 40) (size 4) in 
+
+  let h = sub tempBuffer (size 44) (size 4) in 
+  let r = sub tempBuffer (size 48) (size 4) in 
+  let uh = sub tempBuffer (size 52) (size 4) in 
+
+  let hCube = sub tempBuffer (size 56) (size 4) in 
+
+  move_from_jacobian_coordinates_mixed u1 u2 s1 s2 p q tempBuffer16;
+  Hacl.Impl.P256.PointAdd.compute_common_params_point_add h r uh hCube u1 u2 s1 s2 tempBuffer16; 
+  point_add_if_second_branch_impl_mixed result p q u1 u2 s1 s2 r h uh hCube tempBuffer28;
+
+    let h1 = ST.get() in 
+      let pxD = fromDomain_ (as_nat h0 (gsub p (size 0) (size 4))) in 
+      let pyD = fromDomain_ (as_nat h0 (gsub p (size 4) (size 4))) in 
+      let pzD = fromDomain_ (as_nat h0 (gsub p (size 8) (size 4))) in 
+      let qxD = fromDomain_ (as_nat h0 (gsub q (size 0) (size 4))) in 
+      let qyD = fromDomain_ (as_nat h0 (gsub q (size 4) (size 4))) in 
+      let x3 = as_nat h1 (gsub result (size 0) (size 4)) in 
+      let y3 = as_nat h1 (gsub result (size 4) (size 4)) in 
+      let z3 = as_nat h1 (gsub result (size 8) (size 4)) in 
+
+  lemma_pointAdd_Mixed_ToSpecification pxD pyD pzD qxD qyD x3 y3 z3 (as_nat h1 u1) (as_nat h1 u2) (as_nat h1 s1) (as_nat h1 s2) (as_nat h1 h) (as_nat h1 r)
